all examples

share/steel/examples/pulse/Assert.fst
@@ -1,6 +1,73 @@
 module Assert
 open Pulse.Lib.Pervasives
 
+
+// assume val p : x:int -> v1:int -> v2:int -> vprop
+
+// assume val f : x:int -> #v1:int -> #v2:int{v2 > v1} -> 
+//                 stt unit (p x v1 v2) (fun _ -> emp)
+
+
+// ```pulse
+// fn test (_:unit)
+//   requires p 1 2 4
+//   ensures emp
+//   {
+//     f 1 #2
+//   }
+// ```
+
+
+assume val p : prop
+assume val q : prop
+assume val r : prop
+assume val s : prop
+
+
+open FStar.Tactics
+
+assume
+val pp : vprop
+
+assume
+val test (x:unit) (#[exact (`())] y:unit) (z:unit) : stt unit emp (fun _ -> pp)
+
+#set-options "--debug Assert --debug_level SMTQuery"
+
+
+```pulse
+fn test2 (_:unit)
+  requires emp
+  ensures pp
+  {
+    let _x = test () ();
+    ()
+  }
+```
+(*
+
+assume val l1 : unit -> Lemma (requires p) (ensures q)
+assume val l2 : unit -> Lemma (requires q) (ensures r)
+assume val l3 : unit -> Lemma (requires r) (ensures s)
+
+let l4 () : Lemma (requires p) (ensures r) =
+  l1 ();
+  l2()
+
+```pulse
+ghost
+fn ll3 (_:unit)
+  requires pure p
+  ensures pure s
+  {
+    let x = l1();
+    let y = l2();
+    let z = l3();
+    ()
+  }
+```
+
+
 ```pulse
 fn test_assert (r0 r1: ref nat)
                (#p0 #p1:perm)
