share/steel/examples/pulse/lib/Pulse.Lib.Pervasives.fst
@@ -25,3 +25,16 @@ val perform_atomic
   (f : unit -> stt_atomic is a pre post)
   : stt_atomic is a pre post
 let perform_atomic f = f ()
+  : unit -> stt a pre post
+let perform f () = f ()
+
+(* TEMPORARY! REMOVE! *)
+let inames_ext (is1 is2 : inames)
+  : Lemma (requires forall i. Set.mem i is1 <==> Set.mem i is2)
+          (ensures is1 == is2)
+          [SMTPat (is1 == is2)]
+  = Set.lemma_equal_intro is1 is2
+
+let l1 (is1 : inames)
+  : Lemma (join_inames is1 emp_inames == is1) [SMTPat (join_inames is1 emp_inames)]
+  = Set.lemma_equal_intro (join_inames is1 emp_inames) is1
