share/steel/examples/pulse/Invariant.fst
@@ -1,0 +1,103 @@
+module Invariant
+
+open Pulse.Lib.Pervasives
+open Pulse.Lib.Reference
+
+```pulse
+fn package (r:ref int)
+   requires pts_to r 123
+   returns i : inv (pts_to r 123)
+   ensures emp
+{
+  let i : inv (pts_to r 123) = new_invariant' (pts_to r 123);
+  i
+}
+```
+
+// Fails as it is not atomic
+[@@expect_failure]
+```pulse
+fn test2 (_:unit)
+  requires emp
+  returns v:(v:int{v == 2})
+  ensures emp
+{
+  let r = alloc 123;
+  let i = package r;
+  with_invariants i ensures pure True {
+    r := 124;
+    r := 123;
+    ()
+  };
+  2
+}
+```
+
+#set-options "--error_contexts true"
+#set-options "--print_implicits --print_universes"
+// #set-options "--trace_error"
+
+let test (i:inv emp) = assert  (
+  (add_inv emp_inames i)
+  ==
+  ((join_inames (((add_inv #emp) emp_inames) i)) emp_inames)
+)
+
+#set-options "--ugly"
+ ```pulse
+ ghost
+ fn t0 (_:unit) (i:inv emp)
+   requires emp
+   ensures emp
+   opens (add_inv emp_inames i)
+ {
+   with_invariants i {
+     ()
+   }
+ }
+```
+
+#set-options "--ext pulse:guard_policy=SMTSync"
+#set-options "--debug Invariant --debug_level SMTQuery"
+
+assume val i : inv emp
+
+// ```pulse
+// ghost
+// fn zz (_:unit)
+//   requires emp
+//   ensures emp
+// {
+//   (); ()
+// }
+// ```
+
+(* Using invariants while claiming not to. *)
+[@@expect_failure]
+```pulse
+ghost
+fn t1 (_:unit)
+  requires emp
+  ensures emp
+  opens emp_inames
+{
+  with_invariants i {
+    ()
+  }
+}
+```
+
+(* Fails due to bad scoping *)
+```pulse
+fn t2 (_:unit) (i : inv emp)
+  requires emp
+  returns _:int
+  ensures emp
+  // opens (add_inv emp_inames i)
+{
+  with_invariants i ensures emp {
+    ()
+  };
+  123
+}
+```
