share/steel/examples/pulse/parix/Promises.Examples.fst
@@ -1,0 +1,190 @@
+module Promises.Examples
+
+open Pulse.Lib.Pervasives
+open Promises.Temp
+
+#set-options "--ext pulse:guard_policy=SMTSync"
+#set-options "--print_implicits"
+
+(* Assuming invariants *)
+
+// should be ghost
+assume val mk_inv : p:vprop -> stt (inv p) p (fun _ -> emp)
+
+assume val admit_ghost
+  (#a:Type0) (#pre : vprop) (#post : (a -> vprop))
+  (_:unit)
+  : stt_ghost a emp_inames pre post
+
+type abc = | A | B | C
+
+let invp (b:ref abc) (y:ref int) =
+  exists_ (fun (bb:abc) -> pts_to b #one_half bb ** (if bb = B then pts_to y 42 else emp))
+
+```pulse
+fn test_aux (b : ref abc) (y : ref int)
+  requires pts_to b #one_half B ** invp b y
+  ensures pts_to b #one_half C ** pts_to y 42 ** invp b y
+{
+  unfold invp b y;
+  with bb.
+    assert (pts_to b #one_half bb ** `@(if bb = B then pts_to y 42 else emp));
+
+  assert (pts_to b #one_half B);
+  assert (pts_to b #one_half bb);
+
+  // Automate?
+  pts_to_injective_eq #abc
+        #one_half #one_half
+        #B #bb
+        b;
+
+  assert (pts_to b #one_half (reveal (hide B)) ** pts_to b #one_half (reveal (hide B)));
+
+  gather2 #abc #emp_inames b;
+
+  b := C; // The only non-ghost step
+
+  share2 #_ #emp_inames b;
+
+  rewrite emp
+       as (`@(if false then pts_to y 42 else emp));
+
+  intro_exists (fun (bb:abc) -> pts_to b #one_half bb ** (if bb = B then pts_to y 42 else emp))
+    C;
+
+  assert (pts_to y 42);
+
+  fold invp b y;
+
+  ()
+}
+```
+
+```pulse
+fn test_aux_with_inv (b : ref abc) (y : ref int) (i : inv (invp b y))
+  requires pts_to b #one_half B
+  ensures pts_to b #one_half C ** pts_to y 42
+{
+   with_invariants i {
+     test_aux b y
+   }
+}
+```
+
+let pts_to_b_or_c (b : ref abc) =
+  exists_ (fun (v:abc) -> pts_to b #one_half v ** pure (B? v \/ C? v))
+
+```pulse
+fn test_aux_with_inv2 (b : ref abc) (y : ref int) (i : inv (invp b y))
+  requires pts_to_b_or_c b ** emp
+  ensures pts_to_b_or_c b ** pts_to y 42
+{
+   (* This would be a ghost read.. *)
+   unfold (pts_to_b_or_c b);
+   let v = !b;
+   match v {
+      B -> {
+        with_invariants i ensures pts_to b #one_half C ** pts_to y 42
+        {
+          test_aux b y
+        };
+        assert (exists_ (fun (v:abc) -> pts_to b #one_half v ** pure (B? v \/ C? v)));
+        fold pts_to_b_or_c b;
+        ()
+      }
+      C -> {
+        // Ouch... I thought this was ok, but I don't see how to prove
+        // this case. Maybe the way to go is store some permission
+        // to B in the promise itself.
+        admit ()
+      }
+   }
+}
+```
+
+#set-options "--split_queries always"
+
+
+(* Promising and redeeming in a single func *)
+```pulse
+fn test (b : ref abc) (y : ref int)
+  requires pts_to b A ** pts_to y yy
+  returns x:int
+  ensures pts_to y 42
+{
+  share2 #_ #emp_inames b;
+  assert (pts_to b #one_half A);
+  assert (pts_to b #one_half A ** emp);
+
+  rewrite emp
+       as `@(if false then pts_to y 42 else emp);
+  assert (pts_to b #one_half A ** `@(if A = B then pts_to y 42 else emp));
+
+  assert (exists_ (fun (bb:abc) ->
+             pts_to b #one_half bb ** (if bb = B then pts_to y 42 else emp)));
+
+  fold invp b y;
+  let i = mk_inv (invp b y);
+
+  let pp =
+    make_promise
+      (pts_to_b_or_c b)
+      (pts_to y 42)
+      emp
+      (fun () -> test_aux_with_inv2 b y i);
+
+  y := 42;
+
+  // Set b:=B, keeping the invariant.
+  // FIXME: shouldn't have to talk about promise and y?
+  with_invariants i ensures
+     promise (pts_to_b_or_c b) (pts_to y 42)
+     //** pts_to y 42
+     ** pts_to b #one_half B
+  {
+    unfold invp b y;
+    assert (exists bb. pts_to b #one_half bb ** `@(if bb = B then pts_to y 42 else emp));
+    with ba.
+      assert (pts_to b #one_half ba ** `@(if ba = B then pts_to y 42 else emp));
+
+    assert (pts_to b #one_half A);
+
+    // Automate?
+    pts_to_injective_eq #abc
+          #one_half #one_half
+          #A #ba
+          b;
+
+    assert (pure (ba == A));
+
+    gather2 #_ #emp_inames b;
+    b := B;
+    share2 #_ #emp_inames b;
+
+    assert (pts_to b #one_half B ** `@(if B = B then pts_to y 42 else emp));
+    intro_exists (fun (bb:abc) -> pts_to b #one_half bb ** (if bb = B then pts_to y 42 else emp))
+      B;
+    fold (invp b y);
+    assert (invp b y);
+
+    // Pretty hard to find out to do this.
+    rewrite (`@(if ba = B then pts_to y 42 else emp))
+         as emp;
+
+    assert (pts_to b #one_half B);
+
+    ()
+  };
+
+  assert (pts_to b #one_half B);
+  fold (pts_to_b_or_c b);
+  assert (pts_to_b_or_c b);
+  redeem_promise (pts_to_b_or_c b) (pts_to y 42);
+
+  assert (pts_to y 42);
+  drop_ (pts_to_b_or_c b);
+
+  1234 
+}
+```
