share/steel/examples/pulse/parix/Promises.fst
@@ -1,0 +1,361 @@
+module Promises
+
+open Pulse.Lib.Pervasives
+open Pulse.Lib.SpinLock
+open Pulse.Lib.Stick
+
+let comm_pre (#a:Type0) (#o:inames) (#pre1 #pre2 : vprop) (#post : a -> vprop)
+  (f : stt_ghost a o (pre1 ** pre2) post)
+     : stt_ghost a o (pre2 ** pre1) post
+=
+  sub_stt_ghost _ _ (vprop_equiv_comm _ _)
+                    (intro_vprop_post_equiv _ _ (fun _ -> vprop_equiv_refl _))
+                     f
+
+let comm_post (#a:Type0) (#o:inames) (#pre : vprop) (#post1 #post2 : a -> vprop)
+  (f : stt_ghost a o pre (fun x -> post1 x ** post2 x))
+     : stt_ghost a o pre (fun x -> post2 x ** post1 x)
+=
+  sub_stt_ghost _ _ (vprop_equiv_refl _)
+                    (intro_vprop_post_equiv _ _ (fun _ -> vprop_equiv_comm _ _))
+                     f
+
+(* A promise is just a magic stick that preserves the antecedent. *)
+(* TODO: can this really be a ghost step? would we ever need to allocate invariants
+to redeem? *)
+
+let promise f v = f @==> (f ** v)
+
+(* This should be definable once we fix the inames situation *)
+assume
+val ghost_sub_inv
+  (#a:Type0) (#o1 #o2 : inames) (#pre : vprop) (#post : a -> vprop)
+  (f : stt_ghost a o1 pre post)
+  : Pure (stt_ghost a o2 pre post)
+         (requires Set.subset o1 o2)
+         (ensures fun _ -> True)
+
+let return_promise f v =
+  intro_stick f (f ** v) v
+    (fun os ->
+      let ff : stt_ghost unit emp_inames (f ** v) (fun _ -> f ** v) =
+        return_stt_ghost_noeq () (fun _ -> f ** v)
+      in
+      let ff : stt_ghost unit os (f ** v) (fun _ -> f ** v) =
+        ghost_sub_inv ff
+      in
+      let ff : stt_ghost unit os (v ** f) (fun _ -> f ** v) =
+        comm_pre ff
+      in
+      ff)
+
+let make_promise f v extra k =
+  intro_stick f (f ** v) extra
+    (fun os ->
+      let kk : stt_ghost unit emp_inames (f ** extra) (fun _ -> f ** v) =
+        k ()
+      in
+      let kk : stt_ghost unit os (f ** extra) (fun _ -> f ** v) =
+        ghost_sub_inv kk
+      in
+      let kk : stt_ghost unit os (extra ** f) (fun _ -> f ** v) =
+        comm_pre kk
+      in
+      kk)
+
+let redeem_promise f v =
+  comm_pre (elim_stick f (f ** v))
+
+(* Pulse will currently not recognize calls to anything other than
+top-level names, so this allows to force it. *)
+val now
+  (#a #inames #pre #post : _)
+  (f : unit -> stt_ghost a inames pre post)
+  : unit -> stt_ghost a inames pre post
+let now f () = f ()
+
+```pulse
+ghost
+fn bind_promise_aux
+  (f v1 v2 extra : vprop)
+  (k : (unit -> stt_ghost unit emp_inames (f ** extra ** v1) (fun _ -> f ** promise f v2)))
+  (_:unit)
+  requires f  ** (extra ** promise f v1)
+  returns _:unit
+  ensures f ** v2
+{
+  redeem_promise f v1;
+  now k ();
+  redeem_promise f v2
+}
+```
+
+(* If v1 will hold in the future, and if we can in the future make a
+promise that v2 will hold given v1, then we can promise v2 with the
+same deadline. *)
+```pulse
+ghost
+fn __bind_promise
+  (#f #v1 #v2 : vprop) (extra : vprop)
+  (k : (unit -> stt_ghost unit emp_inames (f ** extra ** v1) (fun _ -> f ** promise f v2)))
+  requires promise f v1 ** extra
+  returns _:unit
+  ensures promise f v2
+{
+  let k
+    : (unit -> stt_ghost unit emp_inames (f ** (extra ** promise f v1))
+                                      (fun _ -> f ** v2))
+    = bind_promise_aux f v1 v2 extra k;
+  make_promise f v2 (extra ** promise f v1)
+      k
+}
+```
+
+let bind_promise #f #v1 #v2 extra k = __bind_promise #f #v1 #v2 extra k
+
+inline_for_extraction
+val frame_stt_ghost_left
+  (#a:Type0)
+  (#opens:inames)
+  (#pre:vprop) (#post:a -> vprop)
+  (frame:vprop)
+  (e:stt_ghost a opens pre post)
+  : stt_ghost a opens (frame ** pre) (fun x -> frame ** post x)
+let frame_stt_ghost_left #a #opens #pre #post frame e =
+  let e : stt_ghost a opens (pre ** frame) (fun x -> post x ** frame) =
+    frame_stt_ghost frame e
+  in
+  let e : stt_ghost a opens (frame ** pre) (fun x -> post x ** frame) =
+    comm_pre e
+  in
+  let e : stt_ghost a opens (frame ** pre) (fun x -> frame ** post x) =
+    comm_post e
+  in
+  e
+
+let bind_promise' #f #v1 #v2 extra k =
+  let k : unit -> stt_ghost unit emp_inames (extra ** v1) (fun _ -> promise f v2) =
+    k
+  in
+  let k : unit -> stt_ghost unit emp_inames (f ** (extra ** v1)) (fun _ -> f ** promise f v2) =
+    fun () -> frame_stt_ghost_left f (k ())
+  in
+  let k : unit -> stt_ghost unit emp_inames (f ** extra ** v1) (fun _ -> f ** promise f v2) =
+    fun () -> sub_stt_ghost _ _ 
+                  (vprop_equiv_sym _ _ (vprop_equiv_assoc _ _ _))
+                  (intro_vprop_post_equiv _ _ (fun _ -> vprop_equiv_refl _))
+                  (k ())
+  in
+  bind_promise #f #v1 #v2 extra k
+
+(* We can define join_promise (NB: very brittle to write this in plain stt *)
+let join_promise (#f:vprop) (v1:vprop) (v2:vprop)
+  : stt_ghost unit
+              emp_inames
+              (promise f v1 ** promise f v2)
+              (fun () -> promise f (v1 ** v2))
+  = bind_promise' (promise f v2) (fun () ->
+    bind_promise' v1 (fun () ->
+    return_promise f (v1 ** v2)))
+
+(* split_promise *)
+#set-options "--ext pulse:guard_policy=SMTSync"
+
+module GR = Pulse.Lib.GhostReference
+
+let inv_p' (f v1 v2 : vprop) (r1 r2 : GR.ref bool) (b1 b2 : bool) =
+     GR.pts_to r1 #one_half b1
+  ** GR.pts_to r2 #one_half b2
+  ** (match b1, b2 with
+      | false, false -> promise f (v1 ** v2)
+      | false, true -> v1
+      | true, false -> v2
+      | true, true -> emp)
+
+let inv_p (f v1 v2 : vprop) (r1 r2 : GR.ref bool) : vprop =
+  exists_ (fun b1 -> exists_ (fun b2 -> inv_p' f v1 v2 r1 r2 b1 b2))
+
+```pulse
+ghost
+fn __elim_l (#f:vprop) (v1:vprop) (v2:vprop) (r1 r2 : GR.ref bool) (i : inv (inv_p f v1 v2 r1 r2)) (_:unit)
+  requires f ** GR.pts_to r1 #one_half false
+  ensures f ** v1
+{
+  open Pulse.Lib.GhostReference;
+  with_invariants i {
+    unfold (inv_p f v1 v2 r1 r2);
+    with bb1 bb2.
+      assert (inv_p' f v1 v2 r1 r2 bb1 bb2);
+    unfold (inv_p' f v1 v2 r1 r2 bb1 bb2);
+    let b1 = !r1;
+    let b2 = !r2;
+
+    assert (pure (b1 == bb1));
+    assert (pure (b2 == bb2));
+
+    gather2 #_ #emp_inames
+      r1
+      #false #b1;
+
+    let b1 : bool = stt_ghost_reveal _ b1;
+    let b2 : bool = stt_ghost_reveal _ b2;
+
+    if b2 {
+      (* The "easy" case: the big promise has already been claimed
+      by the other subpromise, so we just extract our resource. *)
+      assert (pts_to r1 false);
+      r1 := true;
+      rewrite emp ** `@(match false, true with
+                 | false, false -> promise f (v1 ** v2)
+                 | false, true -> v1
+                 | true, false -> v2
+                 | true, true -> emp)
+           as `@(match true, true with
+                 | false, false -> promise f (v1 ** v2)
+                 | false, true -> v1
+                 | true, false -> v2
+                 | true, true -> emp) ** v1;
+
+      (* I don't understand why this remains in the ctx, but get rid
+      of it as it's just emp *)
+      rewrite `@(match true, true with
+                 | false, false -> promise f (v1 ** v2)
+                 | false, true -> v1
+                 | true, false -> v2
+                 | true, true -> emp)
+           as emp;
+
+      share2 #_ #emp_inames r1;
+      fold (inv_p' f v1 v2 r1 r2 true true);
+      fold (inv_p f v1 v2 r1 r2);
+      assert (f ** v1 ** inv_p f v1 v2 r1 r2);
+      drop_ (pts_to r1 #one_half true);
+      ()
+    } else {
+      (* The "hard" case: the big promise has not been claimed.
+      Claim it, split it, and store the leftover in the invariant. *)
+      assert (pts_to r1 false);
+      // assert (pts_to r2 false);
+
+      rewrite `@(match false, false with
+                 | false, false -> promise f (v1 ** v2)
+                 | false, true -> v1
+                 | true, false -> v2
+                 | true, true -> emp)
+           as promise f (v1 ** v2);
+
+      redeem_promise f (v1 ** v2);
+
+      assert (f ** v1 ** v2);
+
+      r1 := true;
+
+      rewrite v2
+           as `@(match true, false with
+                 | false, false -> promise f (v1 ** v2)
+                 | false, true -> v1
+                 | true, false -> v2
+                 | true, true -> emp);
+
+      share2 #_ #emp_inames r1;
+      fold (inv_p' f v1 v2 r1 r2 true false);
+      fold (inv_p f v1 v2 r1 r2);
+      assert (f ** v1 ** inv_p f v1 v2 r1 r2);
+      drop_ (pts_to r1 #one_half true);
+      ()
+    }
+  }
+}
+```
+
+```pulse
+ghost
+fn __elim_r (#f:vprop) (v1:vprop) (v2:vprop) (r1 r2 : GR.ref bool) (i : inv (inv_p f v1 v2 r1 r2)) (_:unit)
+  requires f ** GR.pts_to r2 #one_half false
+  ensures f ** v2
+{
+  (* Analogous to above... *)
+  admit ()
+}
+```
+
+(* Kinda bogus.. this is an unobservable step, not ghost *)
+assume
+val new_invariant_ghost #opened (p:vprop) : stt_ghost (inv p) opened p (fun _ -> emp)
+
+#set-options "--print_implicits --print_universes"
+
+```pulse
+ghost
+fn __split_promise (#f:vprop) (v1:vprop) (v2:vprop)
+  requires promise f (v1 ** v2)
+  ensures promise f v1 ** promise f v2
+{
+   let r1 = GR.alloc false;
+   let r2 = GR.alloc false;
+   GR.share2 #_ #emp_inames r1;
+   GR.share2 #_ #emp_inames r2;
+
+   rewrite (promise f (v1 ** v2))
+        as `@(match false, false with
+            | false, false -> promise f (v1 ** v2)
+            | false, true -> v1
+            | true, false -> v2
+            | true, true -> emp);
+
+  assert (
+     GR.pts_to r1 #one_half false
+  ** GR.pts_to r2 #one_half false
+  ** `@(match false, false with
+      | false, false -> promise f (v1 ** v2)
+      | false, true -> v1
+      | true, false -> v2
+      | true, true -> emp));
+
+  fold (inv_p' f v1 v2 r1 r2 false false);
+  fold (inv_p f v1 v2 r1 r2);
+
+  let i = new_invariant_ghost #emp_inames (inv_p f v1 v2 r1 r2);
+
+  make_promise
+    f
+    v1
+    (GR.pts_to r1 #one_half false)
+    (__elim_l #f v1 v2 r1 r2 i);
+
+  make_promise
+    f
+    v2
+    (GR.pts_to r2 #one_half false)
+    (__elim_r #f v1 v2 r1 r2 i);
+
+  ()
+}
+```
+
+let split_promise (#f:vprop) (v1:vprop) (v2:vprop)
+  : stt_ghost unit
+              emp_inames
+              (promise f (v1 ** v2))
+              (fun () -> promise f v1 ** promise f v2)
+  = __split_promise #f v1 v2
+
+(* /split_promise *)
+
+let rewrite_promise (#f:vprop) (v1 : vprop) (v2 : vprop)
+  (k : unit -> stt_ghost unit emp_inames v1 (fun _ -> v2))
+  : stt_ghost unit
+              emp_inames
+              (promise f v1)
+              (fun _ -> promise f v2)
+= bind_sttg
+    (rewrite (promise f v1) (promise f v1 ** emp)
+       (vprop_equiv_trans _ _ _
+         (vprop_equiv_sym _ _ (vprop_equiv_unit (promise f v1)))
+         (vprop_equiv_comm _ _)))
+    (fun () ->
+      bind_promise' #_ #v1 #_ emp (fun () ->
+        bind_sttg (rewrite (emp ** v1) v1 (vprop_equiv_unit v1)) (fun () ->
+        bind_sttg (k ())
+          (fun () -> return_promise f v2)))
+    )
