share/steel/examples/pulse/parix/Promises.fsti
@@ -1,0 +1,49 @@
+module Promises
+
+open Pulse.Lib.Pervasives
+
+val promise (f:vprop) (v:vprop) : vprop
+
+(* Anything that holds now holds in the future too. *)
+val return_promise (f:vprop) (v:vprop)
+  : stt_ghost unit emp_inames v (fun _ -> promise f v)
+
+val make_promise (f:vprop) (v:vprop) (extra:vprop)
+  ($k : unit -> stt_ghost unit emp_inames (f ** extra) (fun _ -> f ** v))
+  : stt_ghost unit emp_inames extra (fun _ -> promise f v)
+
+val redeem_promise (f:vprop) (v:vprop)
+  : stt_ghost unit emp_inames (f ** promise f v) (fun () -> f ** v)
+
+val bind_promise (#f:vprop) (#v1:vprop) (#v2:vprop)
+        (extra : vprop)
+        (k : unit -> stt_ghost unit emp_inames (f ** extra ** v1) (fun () -> f ** promise f v2))
+  : stt_ghost unit emp_inames (promise f v1 ** extra) (fun () -> promise f v2)
+
+(* Weaker variant, the proof does not use f. It's implement
+by framing k with f and then using the above combinator. Exposing
+only in case it's useful for inference. *)
+val bind_promise' (#f:vprop) (#v1:vprop) (#v2:vprop)
+        (extra : vprop)
+        (k : unit -> stt_ghost unit emp_inames (extra ** v1) (fun () -> promise f v2))
+  : stt_ghost unit emp_inames (promise f v1 ** extra) (fun () -> promise f v2)
+
+val join_promise (#f:vprop) (v1:vprop) (v2:vprop)
+  : stt_ghost unit
+              emp_inames
+              (promise f v1 ** promise f v2)
+              (fun () -> promise f (v1 ** v2))
+
+val split_promise (#f:vprop) (v1:vprop) (v2:vprop)
+  : stt_ghost unit
+              emp_inames
+              (promise f (v1 ** v2))
+              (fun () -> promise f v1 ** promise f v2)
+
+// TODO: write a variant that assumes f too
+val rewrite_promise (#f:vprop) (v1 : vprop) (v2 : vprop)
+  (k : unit -> stt_ghost unit emp_inames v1 (fun _ -> v2))
+  : stt_ghost unit
+              emp_inames
+              (promise f v1)
+              (fun _ -> promise f v2)
